theories/νType/LeInductive.v
@@ -1,5 +1,14 @@
 From Bonak Require Import Notation.
 
+Set Warnings "-notation-overridden".
+Reserved Infix "<=" (at level 70).
+Inductive lePeano p: nat -> Type :=
+  | le_n: p <= p
+  | le_S {n}: p <= n -> p <= n.+1
+where "p <= n" := (lePeano p n): nat_scope.
+
+Arguments le_S {p n} H.
+
 (** An inductive definition of le *)
 Reserved Infix "<~" (at level 70).
 Inductive leI n: nat -> Type :=
@@ -9,7 +18,7 @@ where "p <~ n" := (leI n p): nat_scope.
 
 Arguments leI_down {n p} H.
 
-Lemma leI_up {n p}: n <~ p -> n <~ p.+1.
+Lemma leI_up {p n}: p <~ n -> p <~ n.+1.
   induction 1. constructor. now constructor. now constructor.
 Defined.
 
@@ -17,9 +26,57 @@ Lemma leI_O {p}: O <~ p.
   induction p. now constructor. now apply leI_up.
 Defined.
 
+Lemma le_O {p}: O <= p.
+  induction p. now constructor. now constructor.
+Defined.
+
+Lemma le_O_contra {p}: p.+1 <= O -> False.
+  destruct p. now auto. now auto.
+Defined.
+
+Lemma eq_O_contra {p}: p.+1 = O -> False.
+  now auto.
+Defined.
+
+Lemma le_O_eq {p}: p <= 0 -> p = 0.
+  intro H. destruct p. now trivial. exfalso. now apply le_O_contra in H.
+Defined.
+
+Lemma le_down {p n}: p.+1 <= n -> p <= n.
+  induction 1. constructor; now constructor. now constructor.
+Defined.
+
+Lemma le_up {p n}: p <= n -> p <= n.+1.
+  induction 1. constructor; now constructor. now constructor.
+Defined.
+
+(* Lemma le_lower_both {p n}: p.+1 <= n.+1 -> p <= n.
+  induction 1. apply le_down. now constructor. admit. apply le_up in IHn. now intros _.
+Defined. *)
+
+Lemma leI_le_conversion {p n}: p <~ n -> p <= n.
+  induction 1. now constructor. now apply le_down.
+Defined.
+
+Lemma le_leI_conversion {p n}: p <= n -> p <~ n.
+  induction 1. now constructor. now apply leI_up.
+Defined.
+
+Lemma le_O_eq' {p}: p = 0 -> p <= 0.
+  intro H. destruct p. now constructor. exfalso. now apply eq_O_contra in H.
+Defined.
+
+Lemma leI_O_eq {p}: p <~ 0 -> p = 0.
+  intro H. apply leI_le_conversion in H. now apply le_O_eq.
+Defined.
+
+Lemma leI_O_eq' {p}: p = 0 -> p <~ 0.
+  intro H. apply le_leI_conversion. now apply le_O_eq'.
+Defined.
+
 Lemma leI_O_contra {n}: n.+1 <~ O -> False.
-  intro H.
-Admitted.
+  intro H. now apply leI_le_conversion in H.
+Defined.
 
 Lemma leI_lower_both {n p}: p.+1 <~ n.+1 -> p <~ n.
   intro H. change p with (pred (S p)).
